f2cap: add binding roles to kind environment

devel/Iron/Language/SystemF2Cap/Kind/Ki.v
@@ -19,6 +19,19 @@ Inductive ki : Type :=
 Hint Constructors ki.
 
 
+(* Roles describe how each binding was added to the kind environent. *)
+Inductive role : Type :=
+ (* Type is bound abstractly.
+    Used for type abstractions like with (/\(a : k). x)  *)
+ | OAbs 
+
+ (* Type is bound concretely.
+    Used for private and extension regions, like with (private r with caps in x) 
+    In the expression 'x', the type 'r' refers to a concrete region with
+    specific capabilities. *)
+ | OCon.
+
+
 (* Kind Environments *)
-Definition kienv := list ki.
+Definition kienv := list (role * ki).
 Hint Unfold kienv.
