devel/Iron/Language/SystemF2Cap/Type/Operator/SubstTT.v
@@ -38,48 +38,49 @@ Qed.
    otherwise indices that reference subst type are broken, and 
    the resulting type env would not be well formed *)
 Theorem subst_type_type_ix
- :  forall ix ke sp t1 k1 t2 k2
- ,  get ix ke = Some k2
+ :  forall ix ke sp t1 k1 t2 k2 o2
+ ,  get ix ke = Some (o2, k2)
  -> KindT ke sp t1 k1
  -> KindT (delete ix ke) sp t2 k2
  -> KindT (delete ix ke) sp (substTT ix t2 t1) k1.
 Proof.
- intros. gen ix ke sp t2 k1 k2.
+ intros. gen ix ke sp t2 k1 o2 k2.
  induction t1; intros; simpl; inverts_kind; eauto.
 
- Case "TVar".
-  fbreak_nat_compare.
-  SCase "n = ix".
-   rewrite H in H5.
-   inverts H5. auto.
+ - Case "TVar".
+   fbreak_nat_compare.
+   + SCase "n = ix".
+     destruct H5 as [o].
+     rewrite H in H0.
+     inverts H0. auto.
 
-  SCase "n < ix".
-   apply KiVar. rewrite <- H5.
-   apply get_delete_above; auto.
+   + SCase "n < ix".
+     apply KiVar. shift o. rewrite <- H0.
+     apply get_delete_above; auto.
 
-  SCase "n > ix".
-   apply KiVar. rewrite <- H5.
-   destruct n.
-    burn.
-    simpl. nnat. apply get_delete_below. omega.
+   + SCase "n > ix".
+     apply KiVar. shift o. rewrite <- H0.
+     destruct n.
+     * burn.
+     * simpl. nnat. apply get_delete_below. omega.
 
- Case "TForall".
-  apply KiForall.
-  rewrite delete_rewind.
-  eapply IHt1; eauto.
+ - Case "TForall".
+   apply KiForall.
+   rewrite delete_rewind.
+   eapply IHt1; eauto.
    apply kind_kienv_weaken; auto.
 Qed.
 
 
 Theorem subst_type_type
- :  forall ke sp t1 k1 t2 k2
- ,  KindT (ke :> k2) sp t1 k1
- -> KindT ke         sp t2 k2
+ :  forall ke sp t1 k1 t2 o2 k2
+ ,  KindT (ke :> (o2, k2)) sp t1 k1
+ -> KindT ke               sp t2 k2
  -> KindT ke sp (substTT 0 t2 t1) k1.
 Proof.
  intros.
  unfold substTT.
- rrwrite (ke = delete 0 (ke :> k2)).
+ rrwrite (ke = delete 0 (ke :> (o2, k2))).
  eapply subst_type_type_ix; burn.
 Qed.
 
@@ -87,21 +88,21 @@ Qed.
 (* If two types are equivalent, and we substitute some third type
    into both, then the result is also equivalent. *)
 Lemma substTT_EquivT
- :  forall  ke sp t1 t2 t3 k3 k
- ,  KindT    ke sp t3 k3
- -> EquivT (ke :> k3) sp t1 t2 k
+ :  forall  ke sp t1 t2 t3 o3 k3 k
+ ,  KindT   ke sp t3 k3
+ -> EquivT (ke :> (o3, k3)) sp t1 t2 k
  -> EquivT  ke sp (substTT 0 t3 t1) (substTT 0 t3 t2) k.
 Proof.
- intros ke sp t1 t2 t3 k3 k HK HE.
- have HK1: (KindT (ke :> k3) sp t1 k).
- have HK2: (KindT (ke :> k3) sp t2 k).
- remember (ke :> k3) as X.
+ intros ke sp t1 t2 t3 o3 k3 k HK HE.
+ have HK1: (KindT (ke :> (o3, k3)) sp t1 k).
+ have HK2: (KindT (ke :> (o3, k3)) sp t2 k).
+ remember (ke :> (o3, k3)) as X.
  induction HE; subst.
 
  - Case "EqRefl".
    eapply EqRefl; 
     eauto using subst_type_type.
-  
+
  - Case "EqSym".
    eapply EqSym;
     eauto using subst_type_type.
@@ -125,13 +126,12 @@ Proof.
  - Case "EqSumComm".
    eapply EqSumComm; fold substTT. auto.
    eauto using subst_type_type.
-   eauto using subst_type_type. 
+   eauto using subst_type_type.
 
  - Case "EqSumAssoc".
    eapply EqSumAssoc; fold substTT. auto.
    eauto using subst_type_type.
-   eauto using subst_type_type. 
-   eauto using subst_type_type. 
-Qed.   
-
+   eauto using subst_type_type.
+   eauto using subst_type_type.
+Qed.
 
