devel/Iron/Language/SystemF2Cap/Type/Relation/KindT/WeakKiEnv.v
@@ -4,15 +4,19 @@ Require Export Iron.Language.SystemF2Cap.Type.Relation.KindT.Base.
 
 (* Weaken kind environment in kind judgement. *)
 Lemma kind_kienv_insert
- :  forall ke sp ix t k1 k2
- ,  KindT   ke sp t k1
- -> KindT   (insert ix k2 ke) sp (liftTT 1 ix t) k1.
+ :  forall ke sp ix t k1 k2 o2
+ ,  KindT  ke sp t k1
+ -> KindT  (insert ix (o2, k2) ke) sp (liftTT 1 ix t) k1.
 Proof.
  intros. gen ix ke sp k1.
  induction t; intros; simpl; inverts_kind; eauto.
 
  - Case "TVar".
-   lift_cases; snorm.
+   destruct H3 as [o1].
+   lift_cases.
+   + eapply KiVar. exists o1. snorm.
+   + eapply KiVar. exists o1. snorm.
+   + eapply KiVar. exists o1. snorm.
 
  - Case "TForall".
    apply KiForall.
@@ -21,12 +25,12 @@ Qed.
 
 
 Lemma kind_kienv_weaken
- :  forall ke sp t k1 k2
- ,  KindT   ke sp        t              k1
- -> KindT  (ke :> k2) sp (liftTT 1 0 t) k1.
+ :  forall ke sp t k1 o2 k2
+ ,  KindT   ke sp           t                 k1
+ -> KindT  (ke :> (o2, k2)) sp (liftTT 1 0 t) k1.
 Proof.
  intros.
- rrwrite (ke :> k2 = insert 0 k2 ke).
+ rrwrite (ke :> (o2, k2) = insert 0 (o2, k2) ke).
  apply kind_kienv_insert. auto.
 Qed.
 
